manual proof of the counter example

examples/count/verif.v
@@ -26,7 +26,7 @@ Opaque IdentMap.empty IdentMap.set PathMap.empty PathMap.set.
 (* Global environment *)
 Definition ge := Eval compute in gen_ge prog.
 
-Definition instantiation := Eval compute in instantiate_prog prog.
+Definition instantiation := Eval compute in instantiate_prog ge prog.
 
 (* inst_m *)
 Definition inst_m := Eval compute in fst instantiation.
@@ -39,7 +39,6 @@ Notation path := (list ident).
 
 Transparent IdentMap.empty IdentMap.set PathMap.empty PathMap.set.
 
-Module Experiment.
 Definition this : path := [!"main"; !"ig"].
 Definition init_st : state := (PathMap.empty, init_es).
 
@@ -51,6 +50,8 @@ Definition myFundef := Eval compute in
   | Some x => x
   | None => dummy_fundef
   end.
+
+Module Experiment.
 
 Definition v1 : @ValueBase Info := ValBaseHeader [(!"firstBit", ValBaseBit 1%nat 0)] true.
 Definition v2 : @ValueBase Info := ValBaseStruct [(!"myHeader", v1)].
@@ -80,22 +81,35 @@ Opaque IdentMap.empty IdentMap.set PathMap.empty PathMap.set PathMap.sets.
 Definition st' := Eval compute in (projT1 eval_func).
 Print st'.
 
+End Experiment.
+
 (* Functional model *)
 Notation Val := (@ValueBase Info).
 Notation P4String := (P4String.t Info).
-Definition array_state := (list Z).
+
+
+Module BitArray.
+  Definition t := (list Z).
+
+  Section Operations.
+    Variable (width : positive).
+
+    Definition incr (ast: t) (i: Z) : t :=
+      upd_Znth i ast (BitArith.plus_mod width (Znth i ast) 1).
+
+    Definition incr_sat (ast: t) (i: Z) : t :=
+      upd_Znth i ast (BitArith.plus_sat width (Znth i ast) 1).
+
+  End Operations.
+End BitArray.
+
+
 Definition NUM_ENTRY := 2.
+Definition WIDTH : positive := 4.
 
-Fixpoint array_incr (ast: array_state) (i: nat) : array_state :=
-  match i, ast with
-    | O, hd :: tl => (hd + 1) :: tl
-    | S n, hd :: tl => array_incr tl n
-    | _, [] => ast
-  end.
-
-Definition ast_match (st : state) (ast : array_state) : Prop :=
+Definition ast_match (st : state) (ast : BitArray.t) : Prop :=
   exists content,
-  PathMap.get !["main"; "ig"; "myCounter"] (snd st) = Some (ObjRegister (mk_register 1%nat NUM_ENTRY content)) /\
+  PathMap.get !["main"; "ig"; "myCounter"] (snd st) = Some (ObjRegister (mk_register 4%nat NUM_ENTRY content)) /\
   content = ast.
 
 Definition field_contains (v : Val) (name : P4String) (data: Val) : Prop :=
@@ -105,33 +119,44 @@ Definition field_contains (v : Val) (name : P4String) (data: Val) : Prop :=
   | _ => False
   end.
 
+Definition process (width : positive) (fbit : Z) (ast : BitArray.t) : (BitArray.t * Z) :=
+  if fbit =? 1 then
+    (BitArray.incr width ast 1, 48)
+  else
+    (BitArray.incr width ast 0, 0).
+
 Section Experiment1.
 Variable fbit : Z.
 Variable hdr : Val.
 Variable meta : Val.
 Variable standard_metadata : Val.
-Variable ast : array_state.
+Variable ast : BitArray.t.
 
 Definition pre (* (fbit : Z) (hdr meta standard_metadata : Val) *) (in_args : list Val) (st : state) :=
   in_args = [ValBaseStruct [(!"myHeader", hdr)]; meta; standard_metadata]
-    /\ field_contains hdr !"firstBit" (ValBaseBit 1%nat fbit)
-    /\ ast_match st ast.
-
-Definition process (fbit : Z) (ast : array_state) : (array_state * Z) :=
-  if fbit =? 1 then
-    (array_incr ast 1, 48)
-  else
-    (array_incr ast 0, 0).
+  /\ (exists hdr_fields, hdr = ValBaseHeader hdr_fields true)
+  /\ (exists meta_fields, meta = ValBaseStruct meta_fields)
+  /\ (exists std_meta_fields, standard_metadata = ValBaseStruct std_meta_fields)
+  /\ field_contains hdr !"firstBit" (ValBaseBit 1%nat fbit)
+  /\ (exists counter, field_contains meta !"counter" (ValBaseBit (Z.to_nat (Z.pos WIDTH)) counter))
+  /\ (exists eport, field_contains standard_metadata !"egress_spec" (ValBaseBit 9%nat eport))
+  /\ ast_match st ast.
 
 Definition post (* (fbit : Z) (hdr meta standard_metadata : Val) *) (out_args : list Val) (st : state) :=
-  let (ast', eport) := process fbit ast in
-  exists standard_metadata' std_meta_fields std_meta_fields',
-  out_args = [hdr; meta; standard_metadata']
+  let (ast', eport) := process WIDTH fbit ast in
+  exists standard_metadata' std_meta_fields std_meta_fields' meta_fields meta_fields' meta',
+  out_args = [ValBaseStruct [(!"myHeader", hdr)]; meta'; standard_metadata']
+    /\ meta = ValBaseStruct meta_fields 
+    /\ meta' = ValBaseStruct meta_fields'
+    /\ field_contains meta' !"counter" (ValBaseBit (Z.to_nat (Z.pos WIDTH)) (Znth (if fbit =? 1 then 1 else 0) ast))
+    /\ Ops.eval_binary_op_eq (ValBaseStruct (AList.filter meta_fields (P4String.equivb !"counter" )))
+                             (ValBaseStruct (AList.filter meta_fields' (P4String.equivb !"counter" )))
+       = Some true
     /\ standard_metadata = ValBaseStruct std_meta_fields 
     /\ standard_metadata' = ValBaseStruct std_meta_fields'
     /\ field_contains standard_metadata' !"egress_spec" (ValBaseBit 9%nat eport)
     /\ Ops.eval_binary_op_eq (ValBaseStruct (AList.filter std_meta_fields (P4String.equivb !"egress_spec" )))
-                         (ValBaseStruct (AList.filter std_meta_fields' (P4String.equivb !"egress_spec" )))
+                             (ValBaseStruct (AList.filter std_meta_fields' (P4String.equivb !"egress_spec" )))
        = Some true
     /\ ast_match st ast'.
 
@@ -140,4 +165,256 @@ Abort.
 
 End Experiment1.
 
-End Experiment.
+
+Section Experiment2.
+
+(*Assumption argsassertion:= (in_args : list Val) (st : state)*)
+Definition ArgAssertion (T:Type) := forall (t:T), arg_assertion.
+
+Record FunSpec := {
+  WITHtype : Type;
+  preCond: ArgAssertion WITHtype ;
+  postCond: ArgAssertion WITHtype ;
+}.
+
+(* As general as possible *)
+Definition pre2 : ArgAssertion (Z * Val * Val * Val * BitArray.t) :=
+ fun t in_args st =>
+   match t with (fbit, hdr, meta, standard_metadata, ast) =>
+    in_args = [ValBaseStruct [(!"myHeader", hdr)]; meta; standard_metadata]
+   /\ (exists hdr_fields, hdr = ValBaseHeader hdr_fields true)
+   /\ (exists meta_fields, meta = ValBaseStruct meta_fields)
+   /\ (exists std_meta_fields, standard_metadata = ValBaseStruct std_meta_fields)
+   /\ field_contains hdr !"firstBit" (ValBaseBit 1%nat fbit)
+   /\ (exists counter, field_contains meta !"counter" (ValBaseBit (Z.to_nat (Z.pos WIDTH)) counter))
+   /\ (exists eport, field_contains standard_metadata !"egress_spec" (ValBaseBit 9%nat eport))
+   /\ ast_match st ast
+ end.
+
+(* As precise as possible *)
+Definition post2 : ArgAssertion (Z * Val * Val * Val * BitArray.t) :=
+  fun t out_args st =>
+  match t with (fbit, hdr, meta, standard_metadata, ast) =>
+  let (ast', eport) := process WIDTH fbit ast in
+  exists standard_metadata' std_meta_fields std_meta_fields' meta_fields meta_fields' meta',
+  out_args = [ValBaseStruct [(!"myHeader", hdr)]; meta'; standard_metadata']
+    /\ meta = ValBaseStruct meta_fields 
+    /\ meta' = ValBaseStruct meta_fields'
+    /\ field_contains meta' !"counter" (ValBaseBit (Z.to_nat (Z.pos WIDTH)) (Znth (if fbit =? 1 then 1 else 0) ast))
+    /\ Ops.eval_binary_op_eq (ValBaseStruct (AList.filter meta_fields (P4String.equivb !"counter" )))
+                             (ValBaseStruct (AList.filter meta_fields' (P4String.equivb !"counter" )))
+       = Some true
+    /\ standard_metadata = ValBaseStruct std_meta_fields 
+    /\ standard_metadata' = ValBaseStruct std_meta_fields'
+    /\ field_contains standard_metadata' !"egress_spec" (ValBaseBit 9%nat eport)
+    /\ Ops.eval_binary_op_eq (ValBaseStruct (AList.filter std_meta_fields (P4String.equivb !"egress_spec" )))
+                             (ValBaseStruct (AList.filter std_meta_fields' (P4String.equivb !"egress_spec" )))
+       = Some true
+    /\ ast_match st ast'
+  end.
+
+Definition countFunspec : FunSpec := {| WITHtype := (Z * Val * Val * Val * BitArray.t)%type;
+                                       preCond := pre2;
+                                       postCond := post2 |}.
+
+
+Definition statement := Eval compute in
+  match myFundef with
+  | FInternal vals init (BlockCons stmt' rest') => stmt'
+  | _ => empty_statement
+  end.
+
+Ltac inv H := inversion H; subst; clear H.
+Transparent IdentMap.empty IdentMap.set PathMap.empty PathMap.set PathMap.sets.
+Set Printing Notations.
+
+Lemma body_counter : forall t : WITHtype countFunspec,
+     hoare_func ge inst_m this (preCond countFunspec t) myFundef nil (postCond countFunspec t).
+Proof.
+  intros t.
+  unfold countFunspec in t.
+  simpl in t.
+  destruct t as [[[[fbit hdr] meta] standard_metadata] ast].
+  simpl.
+  unfold pre2.
+  unfold hoare_func.
+  intros.
+  destruct st, st'.
+  (* +[H16] exec_func on ingress.apply() *)
+  inv H0.
+  destruct H as [A [[hdr_fields B] [[meta_fields C] 
+                [[std_meta_fields D] [E [[counter F] [[eport G] [content [J K]]]]]]]]].
+  unfold default, Inhabitant_Info in *.
+  simpl in *.
+  rewrite A in H4.
+  inv H4. inv H5. inv H6. 
+  (* +[H7] exec_block*)
+  inv H10. inv H4. inv H11. inv H9. inv H8.
+  inv H9. inv H8. inv H14. inv H0.
+  inv H11. inv H4.
+  rewrite E in H.
+  inv H. inv H10. inv H8. inv H9. inv H11.
+  inversion H13. clear H13.
+  destruct b.
+  (* true: forward packets *)
+  - inv H12. 
+    (* +[H10] exec_block *)
+    inv H9. inv H5.
+    (* +[H18] exec_call on do_forward() *)
+    inv H12. inv H14. inv H9. inv H3.
+    inv H12. inv H13. inv H14.
+    inv H11. inv H15. 
+    (* +[H20] exec_func on do_forward() *)
+    inv H17. inv H3. inv H4. inv H5. 
+    (* +[H9] exec_block *)
+    inv H11. inv H5.
+    (* +[H21] exec_call on register.read() *)
+    inv H13. inv H15. 
+    inv H11. inv H3. inv H14. inv H15.
+    inv H12. inv H11. inv H3.
+    inv H12. inv H14. inv H15.
+    inv H13. inv H17. inv H19.
+    inv H14. inv H.
+    rewrite J in H2. inv H2. clear H4.
+    (* -[H21] *)
+    inv H21. inv H8. inv H3. inv H5. inv H6.
+    inv H12. apply AList.get_some_set with 
+              (v2:=(ValBaseBit 4 (Znth (BitArith.mod_bound 32 1) ast))) in F.
+    rewrite F in H1. inv H1.
+    inv H13. inv H11.
+    (* -[H9] *)
+    (* +[H11]: exec_block *)
+    simpl in *. inv H9. inv H5.
+    (* +[H21]: exec_call on register.write() *)
+    inv H13. inv H15. inv H9. inv H3.
+    inv H13. inv H14. inv H15. inv H12.
+    inv H9. inv H3. inv H14. inv H9.
+    inv H14. inv H12. rewrite AList.set_some_get in H1.
+    inv H1. inv H15. inv H9. inv H12. inv H14. inv H22.
+    inv H13. inv H17. inv H19. inv H14.
+    inv H. rewrite J in H4. inv H4. clear H8. clear H9.
+    (* -[H21] *)
+    inv H21.
+    (* -[H11] *)
+    (* +[H9]: exec_block *)
+    inv H11. inv H5.
+    2: inv H11.
+    inv H13. inv H11. inv H14. inv H12.
+    inv H13. inv H15. inv H11. inv H4.
+    inv H6. inv H8. apply AList.get_some_set with 
+                  (v2:=(ValBaseBit 9 (BitArith.mod_bound 9 48))) in G.
+    rewrite G in H1. inv H1.
+    (* -[H9] *)
+    inv H9.
+    (* -[H20] *)
+    inv H20.
+    (* -[H18] *)
+    inv H18.
+    (* -[H10] *)
+    inv H10.
+    (* -[H7] *)
+    inv H7. 
+    (* -[H16] *)
+    inv H16. clear dirs. clear dirs0. clear dirs1.
+    simpl.
+    split. reflexivity.
+    unfold process.
+    apply Z.eqb_eq in H0.
+    subst. simpl. do 6 eexists.
+    split. f_equal. f_equal. 
+    split. reflexivity.
+    split. reflexivity.
+    split. apply AList.set_some_get.
+    split. admit.
+    split. reflexivity.
+    split. reflexivity.
+    split. apply AList.set_some_get.
+    split. admit.
+    unfold ast_match.
+    eexists. simpl.
+    split. 2: reflexivity.
+    unfold PathMap.get, PathMap.set, FuncAsMap.get, FuncAsMap.set.
+    simpl. unfold BitArray.incr. reflexivity.
+  - inv H12. 
+    (* +[H10] exec_block *)
+    inv H9. inv H5.
+    (* +[H18] exec_call on do_forward() *)
+    inv H12. inv H14. inv H15. 
+    (* +[H20] exec_func on do_forward() *)
+    inv H17. inv H3. inv H4. inv H5. 
+    (* +[H9] exec_block *)
+    inv H11. inv H5.
+    (* +[H21] exec_call on register.read() *)
+    inv H13. inv H15. 
+    inv H11. inv H3. inv H14. inv H15.
+    inv H12. inv H11. inv H3.
+    inv H12. inv H14. inv H15.
+    inv H13. inv H17. inv H19.
+    inv H14. inv H.
+    rewrite J in H2. inv H2. clear H4.
+    (* -[H21] *)
+    inv H21. inv H8. inv H3. inv H5. inv H6.
+    inv H12. apply AList.get_some_set with 
+              (v2:=(ValBaseBit 4 (Znth (BitArith.mod_bound 32 0) ast))) in F.
+    rewrite F in H1. inv H1.
+    inv H13. inv H11.
+    (* -[H9] *)
+    (* +[H11]: exec_block *)
+    simpl in *. inv H9. inv H5.
+    (* +[H21]: exec_call on register.write() *)
+    inv H13. inv H15. inv H9. inv H3.
+    inv H13. inv H14. inv H15. inv H12.
+    inv H9. inv H3. inv H14. inv H9.
+    inv H14. inv H12. rewrite AList.set_some_get in H1.
+    inv H1. inv H15. inv H9. inv H12. inv H14. inv H22.
+    inv H13. inv H17. inv H19. inv H14.
+    inv H. rewrite J in H4. inv H4. clear H8. clear H9.
+    (* -[H21] *)
+    inv H21.
+    (* -[H11] *)
+    (* +[H9]: exec_block *)
+    inv H11. inv H5.
+    2: inv H11.
+    inv H13. inv H11. inv H12. inv H17.
+    inv H14. inv H12. inv H13.
+    inv H15. inv H4. inv H6.
+    inv H8.
+    apply AList.get_some_set with 
+          (v2:=(ValBaseBit 9 (BitArith.mod_bound 9 0))) in G.
+    rewrite G in H1. inv H1. inv H11.
+    (* -[H9] *)
+    inv H9.
+    (* -[H20] *)
+    inv H20.
+    (* -[H18] *)
+    inv H18.
+    (* -[H10] *)
+    inv H10.
+    (* -[H7] *)
+    inv H7. 
+    (* -[H16] *)
+    inv H16. clear dirs. clear dirs0. clear dirs1.
+    simpl.
+    split. reflexivity.
+    unfold process.
+    assert (BitArith.mod_bound 1 1 = 1). { reflexivity. }
+    rewrite H in H0.
+    rewrite H0. do 6 eexists.
+    split. f_equal. f_equal. 
+    split. reflexivity.
+    split. reflexivity.
+    split. simpl. apply AList.set_some_get.
+    split. admit.
+    split. reflexivity.
+    split. reflexivity.
+    split. apply AList.set_some_get.
+    split. admit.
+    unfold ast_match.
+    eexists. simpl.
+    split. 2: reflexivity.
+    unfold PathMap.get, PathMap.set, FuncAsMap.get, FuncAsMap.set.
+    simpl. unfold BitArray.incr. reflexivity.
+Admitted.
+
+End Experiment2.
+
